\documentclass{article}
\usepackage{amsmath}
\begin{document}

\section{Switched Lennard-Jones potential}

The potential $u(r)$ is switched from $r = r_s$ to zero $r = r_c$.
\[
  u(r) = \sum_4^7 a_k (r - r_c)^k.
\]
At $r = r_c$, $u = u' = u'' = u''' = 0$;
at $r = r_s$, $u$, $u'$, $u''$, $u'''$ are the same as those at
\[
  u_{LJ}(r) = 4 (r^{-12} - r^{-6}).
\]
The coefficients $a_4, a_5, a_6, a_7$ are 
\begin{align}
  a_4 &= 4 (35 r_s^3 A + 90 r_s^2 \Delta r B + 15 r_s \Delta r^2 C + 28 \Delta r^3 D)/(\Delta r^4 r_s^15), \\
  a_5 &= -24 (14 r_s^3 A + 39 r_s^2 \Delta r B + 7 r_s \Delta r^2 C + 14 \Delta r^3 D)/(\Delta r^5 r_s^15), \\
  a_6 &= 4 (70 r_s^3 A + 20 r_s^2 \Delta r B + 39 r_s \Delta r^2 C + 84 \Delta r^3 D)/(\Delta r^6 r_s^15), \\
  a_7 & = -16 (5 r_s^3 A + 15 r_s^2 \Delta r B + 3 r_s \Delta r^2 C + 7 \Delta r^3 D)/(\Delta r^7 r_s^15),
\end{align}
where $\Delta r = r_c - r_s$, 
$A = 1 - r_s^6$,
$B = 2 - r_s^6$,
$C = 26 - 7 r_s^6$,
$D = 13 - 2 r_s^6$.


\section{Derivates of the energy distribution $\rho(E)$}
For a canonical ensemble, $\rho(E)$,
\begin{align}
\frac {\partial \ln \rho} 
      {\partial E}
    & = \langle \nabla \cdot \mathbf v \rangle_E - \beta, \\
\frac {\partial^2 \ln \rho}
      {\partial E^2}
    & = \langle \mathbf v \cdot \nabla (\nabla \cdot \mathbf v) \rangle_E
      + \langle \Delta (\nabla \cdot \mathbf v)^2 \rangle_E.
\end{align}
where $\mathbf v = \nabla U/(\nabla U \cdot \nabla U)$.


\subsection{Explicit formulas}

The divergence, $\nabla \cdot \mathbf v$,
\begin{align*}
\nabla \cdot \mathbf v
     = \frac { \nabla^2 U }
              { \nabla U \cdot \nabla U }
      - \frac { 2 \nabla U \cdot \nabla \nabla U \cdot \nabla U }
              { (\nabla U \cdot \nabla U)^2 }
     = \frac { L }
              { \mathbf g^2 }
      - \frac { M }
              { (\mathbf g^2)^2 }
\end{align*}
Thus, we need to compute $\mathbf g = \nabla U$, 
$L = \nabla^2 U$, and $M = 2 \mathbf g \cdot \nabla \nabla U \cdot \mathbf g$.

The second $\mathbf v \cdot \nabla (\nabla \cdot \mathbf v)$
\begin{align*}
\mathbf v \cdot \nabla (\nabla \cdot \mathbf v)
    = &  \frac { \mathbf v \cdot \nabla L }
              { \mathbf g^2 }
      - \frac { L (2 \mathbf v \cdot \nabla \nabla U \cdot \mathbf g) }
              { (\mathbf g^2)^2 }
     - \frac { \mathbf v \cdot \nabla M }
              { (\mathbf g^2)^2 } 
      + \frac { M (2 \mathbf v \cdot 2 \nabla \nabla U \cdot \mathbf g)}
              { (\mathbf g^2)^3 } 
\\
   = & \frac { \mathbf g \cdot \nabla L }
              { (\mathbf g^2)^2 }
      - \frac { L M }
              { (\mathbf g^2)^3 }
     - \frac { 4 \mathbf g \cdot \nabla \nabla U \cdot \nabla \nabla U \cdot \mathbf g }
              { (\mathbf g^2)^3 } 
      - \frac { 2 \mathbf g \mathbf g : \nabla \nabla \nabla U \cdot \mathbf g }
              { (\mathbf g^2)^3 } 
      + \frac { 2 M^2}
              { (\mathbf g^2)^4 } 
\\
   = & \frac { \mathbf g \cdot \nabla L }
              { (\mathbf g^2)^2 }
     - \frac { L M + \mathbf h^2  + 2 \mathbf g \mathbf g : \nabla \nabla \nabla U \cdot \mathbf g}
              { (\mathbf g^2)^3 } 
      + \frac { 2 M^2}
              { (\mathbf g^2)^4 },
\end{align*}
where $\mathbf h = 2 \mathbf g \cdot \nabla \nabla U$.

The last $\mathbf r \cdot \nabla (\nabla \cdot \mathbf v)$
\begin{align*}
\mathbf r \cdot \nabla (\nabla \cdot \mathbf v)
    = &  \frac { \mathbf r \cdot \nabla L }
              { \mathbf g^2 }
      - \frac { L (2 \mathbf r \cdot \nabla \nabla U \cdot \mathbf g) }
              { (\mathbf g^2)^2 }
     - \frac { \mathbf r \cdot \nabla M }
              { (\mathbf g^2)^2 } 
      + \frac { M (2 \mathbf r \cdot 2 \nabla \nabla U \cdot \mathbf g)}
              { (\mathbf g^2)^3 } 
\\
   = & \frac { \mathbf r \cdot \nabla L }
              { \mathbf g^2 }
      - \frac { L (\mathbf r \cdot \mathbf h) }
              { (\mathbf g^2)^2 }
     - \frac { \mathbf h \cdot \mathbf s }
              { (\mathbf g^2)^2 } 
      - \frac { 2 \mathbf g \mathbf g : \nabla \nabla \nabla U \cdot \mathbf r }
              { (\mathbf g^2)^2 } 
      + \frac { 2 M (\mathbf r \cdot \mathbf h)}
              { (\mathbf g^2)^3 } 
\\
   = & \frac { \mathbf r \cdot \nabla L }
              { \mathbf g^2 }
     - \frac { L (\mathbf r \cdot \mathbf h) + \mathbf h \cdot \mathbf s + 2 \mathbf g \mathbf g : \nabla \nabla \nabla U \cdot \mathbf r}
              { (\mathbf g^2)^2 }
      + \frac { 2 M (\mathbf r \cdot \mathbf h)}
              { (\mathbf g^2)^3 },
\end{align*}
where $\mathbf s = 2 \mathbf r \cdot \nabla \nabla U$.



\subsection{Compute quantities in terms of a pair potential}

Definition
\begin{align*}
  \phi(r) & = u'(r)/r \\
  \psi(r) & = \phi'(r)/r \\
  \xi(r)  & = \psi'(r)/r
\end{align*}



\subsubsection{The laplacian $L$}
\begin{align*}
L = \nabla^2 U 
  = \sum_k \nabla_k^2 U
  = \sum_{(i, j)} \sum_k \nabla_k^2 u(r_{ij})
  = \sum_{(i, j)} (\nabla_i^2 u(r_{ij}) + \nabla_j^2 u(r_{ij}))
\end{align*}
To expand, 
\begin{align*}
\nabla_i u(r_{ij}) 
& = \phi(r_{ij}) \, \mathbf r_{ij}, \\
\nabla_i^2 u(r_{ij})
& = \nabla_i \phi(r_{ij}) \cdot \mathbf r_{ij} + d \phi(r_{ij})
= \psi(r_{ij}) \, r_{ij}^2  + d \phi(r_{ij}), \\
L = \sum_{(i, j)} L_{ij} & = \sum_{(i, j)} 2 [ \psi(r_{ij}) r_{ij}^2 + d \phi(r_{ij}) ].
\end{align*}
$d = 3$ for the 3D case.



\subsubsection{$\mathbf g \cdot \nabla L$}

\begin{align*}
\nabla_k L = \delta_{ik} \nabla_i L_{ij} + \delta_{jk} \nabla_j L_{ij}. 
\end{align*}
where $\nabla_i L_{ij} = 2 [ \xi(r_{ij}) r_{ij}^2 + 2 \psi(r_{ij}) + d \psi(r_{ij}) ] \mathbf r_{ij}$.
\begin{align*}
\mathbf g \cdot \nabla L
= \sum_k \mathbf g_k \cdot \nabla_k L
= \sum_{(i, j)} 2 [ \xi(r_{ij}) r_{ij}^2 + (2 + d) \psi(r_{ij}) ] (\mathbf r_{ij} \cdot \mathbf g_{ij}),
\end{align*}
where $\mathbf g_{ij} = \mathbf g_i - \mathbf g_j$.



\subsubsection{$\mathbf h = 2 \mathbf g \cdot \nabla \nabla U$}

\begin{align*}
\mathbf h_k &= 2 \mathbf g \cdot \nabla \nabla U
  = 2 \sum_l \mathbf g_l \cdot \nabla_k \nabla_l U
  = 2 \sum_{(i, j)} \sum_l \mathbf g_l \cdot \nabla_k \nabla_l u(r_{ij})
\\
  &= 2 \sum_{(i, j)} \sum_l \mathbf g_l \cdot \nabla_k 
    (\delta_{il} - \delta_{jl}) \, \phi(r_{ij}) \mathbf r_{ij} 
  = 2 \sum_{(i, j)} \mathbf g_{ij} \cdot \nabla_k 
    \, \phi(r_{ij}) \mathbf r_{ij}
\\
  &= 2 \sum_{(i, j)} \mathbf g_{ij} \cdot 
    (\delta_{ik} - \delta_{jk}) \, 
    [\psi(r_{ij}) \mathbf r_{ij} \mathbf r_{ij}
    + \phi(r_{ij}) \mathbf I_{ij}]
\\
  &= 2 (\delta_{ik} - \delta_{jk}) 
      \sum_{(i, j)} [\psi(r_{ij}) (\mathbf g_{ij} \cdot \mathbf r_{ij}) \mathbf r_{ij}
    + \phi(r_{ij}) \mathbf g_{ij}]
\end{align*}



\subsubsection{$\mathbf s = 2 \mathbf r \cdot \nabla \nabla U$}

\begin{align*}
\mathbf s_k &= 2 \mathbf r \cdot \nabla \nabla U
  = 2 \sum_l \mathbf r_l \cdot \nabla_k \nabla_l U
  = 2 \sum_{(i, j)} \sum_l \mathbf x_l \cdot \nabla_k \nabla_l u(r_{ij})
\\
  &= 2 \sum_{(i, j)} \sum_l \mathbf r_l \cdot \nabla_k 
    (\delta_{il} - \delta_{jl}) \, \phi(r_{ij}) \mathbf r_{ij} 
  = 2 \sum_{(i, j)} \mathbf r_{ij} \cdot \nabla_k 
    \, \phi(r_{ij}) \mathbf r_{ij}
\\
  &= 2 \sum_{(i, j)} \mathbf r_{ij} \cdot 
    (\delta_{ik} - \delta_{jk}) \, 
    [\psi(r_{ij}) \mathbf r_{ij} \mathbf r_{ij}
    + \phi(r_{ij}) \mathbf I_{ij}]
\\
  &= 2 (\delta_{ik} - \delta_{jk}) 
      \sum_{(i, j)} [\psi(r_{ij}) r_{ij}^2 + \phi(r_{ij}) ] \mathbf r_{ij}
\end{align*}



\subsubsection{$M = 2 \mathbf g \mathbf g : \nabla \nabla U = \mathbf g \cdot \mathbf h$}

\begin{align*}
M &= \mathbf g \cdot \mathbf h
\\
  &= 2 \sum_{(i, j)} \sum_k (\delta_{ik} - \delta_{jk}) 
    \mathbf g_k \cdot [\psi(r_{ij}) (\mathbf g_{ij} \cdot \mathbf r_{ij}) \mathbf r_{ij}
    + \phi(r_{ij}) \mathbf g_{ij}]
\\
  &= 2 \sum_{(i, j)} 
    \mathbf g_{ij} \cdot [\psi(r_{ij}) (\mathbf g_{ij} \cdot \mathbf r_{ij}) \mathbf r_{ij}
    + \phi(r_{ij}) \mathbf g_{ij}]
\\
  &= 2 \sum_{(i, j)} 
    [\psi(r_{ij}) (\mathbf r_{ij} \cdot \mathbf g_{ij})^2 + \phi(r_ij)\, \mathbf g_{ij}^2].
\end{align*}



\subsubsection{$N = \mathbf g \mathbf g : \nabla \nabla \nabla U \cdot \mathbf g$}

\begin{align*}
N =& \mathbf g \mathbf g : \nabla \nabla \nabla U \cdot \mathbf g
  = \sum_{k, l, m} \mathbf g_k \mathbf g_l : \nabla_k \nabla_l \nabla_m U \cdot \mathbf g_m
\\
  =& \sum_{(i, j)} \sum_{k, l, m} \mathbf g_k \mathbf g_l : \nabla_k \nabla_l \nabla_m u(r_{ij}) \cdot \mathbf g_m
\\
  =& \sum_{(i, j)} \sum_{k, l, m} \mathbf g_k \mathbf g_l : [\nabla_k \nabla_l
    (\delta_{im} - \delta_{jm}) \, \phi(r_{ij}) \mathbf r_{ij}] \cdot \mathbf g_m
\\
  =& \sum_{(i, j)} \sum_{k, l} \mathbf g_k \mathbf g_l : [\nabla_k \nabla_l 
    \, \phi(r_{ij}) \mathbf r_{ij}] \cdot \mathbf g_{ij}
\\
  =& \sum_{(i, j)} \sum_{k, l} \mathbf g_k \mathbf g_l : 
    (\delta_{il} - \delta_{jl}) \, 
    \{
    \nabla [\psi(r_{ij}) \mathbf r_{ij} \mathbf r_{ij}
    + \phi(r_{ij}) \mathbf I_{ij}] 
    \}
  \cdot \mathbf g_{ij}
\\
  =& \sum_{(i, j)} \sum_k \mathbf g_k \mathbf g_{ij} : 
    \{
    \nabla_k [\psi(r_{ij}) \mathbf r_{ij} \mathbf r_{ij}
    + \phi(r_{ij}) \mathbf I_{ij}] 
    \}
  \cdot \mathbf g_{ij}
\\
  =& \sum_{(i, j)} \sum_k \mathbf g_k \mathbf g_{ij} : 
    \{
    (\delta_{ik} - \delta_{jk}) 
    [
    \xi(r_{ij}) \mathbf r_{ij} \mathbf r_{ij} \mathbf r_{ij}
   + \psi(r_{ij}) (\mathbf I_{ij} \mathbf r_{ij}
    + \mathbf I_{ij}^{(13)} \mathbf r_{ij}
    + \mathbf r_{ij} \mathbf I_{ij} ) ] 
    \}
  \cdot \mathbf g_{ij}
\\
  =& \sum_{(i, j)} \mathbf g_{ij} \mathbf g_{ij} : 
    [
    \xi(r_{ij}) \mathbf r_{ij} \mathbf r_{ij} \mathbf r_{ij}
    + \psi(r_{ij}) (\mathbf I_{ij} \mathbf r_{ij}
    + \mathbf I_{ij}^{(13)} \mathbf r_{ij}
    +  \mathbf r_{ij} \mathbf I_{ij})] 
  \cdot \mathbf g_{ij}
\\
  =& \sum_{(i, j)} [
    \xi(r_{ij}) (\mathbf g_{ij} \cdot \mathbf r_{ij})^2
    + 3 \, \psi(r_{ij}) (\mathbf g_{ij} \cdot \mathbf g_{ij})] (\mathbf g_{ij} \cdot \mathbf r_{ij}) 
\end{align*}

\end{document}
